Datatype for intervals.

HOL/DataStrs/Interval_Tree.thy
@@ -5,12 +5,37 @@ begin
 definition max3 :: "('a::ord) \<Rightarrow> 'a \<Rightarrow> 'a \<Rightarrow> 'a" where [rewrite]:
   "max3 a b c = max a (max b c)"
 
+section {* Definition of interval *}
+
+datatype 'a interval = Interval (low: 'a) (high: 'a)
+setup {* add_rewrite_rule_back @{thm interval.collapse} *}
+setup {* add_rewrite_rule @{thm interval.case} *}
+setup {* fold add_rewrite_rule @{thms interval.sel} *}
+
+instantiation interval :: (linorder) linorder begin
+
+definition less: "(a < b) = (low a < low b | (low a = low b \<and> high a < high b))"
+definition less_eq: "(a \<le> b) = (low a < low b | (low a = low b \<and> high a \<le> high b))"
+
+instance proof
+  fix x y z :: "'a interval"
+  show a: "(x < y) = (x \<le> y \<and> \<not> y \<le> x)"
+    using less local.less_eq by force
+  show b: "x \<le> x"
+    by (simp add: local.less_eq)
+  show c: "x \<le> y \<Longrightarrow> y \<le> z \<Longrightarrow> x \<le> z"
+    by (smt Interval_Tree.less_eq dual_order.trans less_trans)
+  show d: "x \<le> y \<Longrightarrow> y \<le> x \<Longrightarrow> x = y"
+    using Interval_Tree.less_eq a interval.expand less by fastforce
+  show e: "x \<le> y \<or> y \<le> x"
+    by (meson Interval_Tree.less_eq leI not_less_iff_gr_or_eq)
+qed end
+
 section {* Definition of an interval tree *}
 
-(* low is the key, high is the value, max is additional info  *)
 datatype interval_tree =
    Tip
- | Node (lsub: interval_tree) (val: "nat \<times> nat") (tmax: nat) (rsub: interval_tree)
+ | Node (lsub: interval_tree) (val: "nat interval") (tmax: nat) (rsub: interval_tree)
 where
   "tmax Tip = 0"
 
@@ -22,24 +47,19 @@ setup {* add_var_induct_rule @{thm interval_tree.induct} *}
 
 section {* Inorder traversal, and set of elements of a tree *}
 
-fun in_traverse_keys :: "interval_tree \<Rightarrow> nat list" where
-  "in_traverse_keys Tip = []"
-| "in_traverse_keys (Node l it m r) = (in_traverse_keys l) @ [fst it] @ (in_traverse_keys r)"
-setup {* fold add_rewrite_rule @{thms in_traverse_keys.simps} *}
-
-fun in_traverse :: "interval_tree \<Rightarrow> (nat \<times> nat) list" where
+fun in_traverse :: "interval_tree \<Rightarrow> nat interval list" where
   "in_traverse Tip = []"
 | "in_traverse (Node l it m r) = (in_traverse l) @ [it] @ (in_traverse r)"
 setup {* fold add_rewrite_rule @{thms in_traverse.simps} *}
 
-fun tree_set_keys :: "interval_tree \<Rightarrow> nat set" where
-  "tree_set_keys Tip = {}"
-| "tree_set_keys (Node l it m r) = {fst it} \<union> tree_set_keys l \<union> tree_set_keys r"
-setup {* fold add_rewrite_rule @{thms tree_set_keys.simps} *}
+fun tree_set :: "interval_tree \<Rightarrow> nat interval set" where
+  "tree_set Tip = {}"
+| "tree_set (Node l it m r) = {it} \<union> tree_set l \<union> tree_set r"
+setup {* fold add_rewrite_rule @{thms tree_set.simps} *}
 
 fun tree_sorted :: "interval_tree \<Rightarrow> bool" where
   "tree_sorted Tip = True"
-| "tree_sorted (Node l it m r) = ((\<forall>x\<in>tree_set_keys l. x < fst it) \<and> (\<forall>x\<in>tree_set_keys r. fst it < x)
+| "tree_sorted (Node l it m r) = ((\<forall>x\<in>tree_set l. x < it) \<and> (\<forall>x\<in>tree_set r. it < x)
                                    \<and> tree_sorted l \<and> tree_sorted r)"
 setup {* add_property_const @{term tree_sorted} *}
 setup {* fold add_rewrite_rule @{thms tree_sorted.simps} *}
@@ -48,43 +68,30 @@ lemma tree_sorted_lr [forward]:
   "tree_sorted (Node l it m r) \<Longrightarrow> tree_sorted l \<and> tree_sorted r" by auto2
 
 lemma inorder_preserve_set [rewrite_back]:
-  "set (in_traverse_keys t) = tree_set_keys t"
+  "set (in_traverse t) = tree_set t"
 @proof @induct t @qed
 
-lemma inorder_keys_sorted [rewrite_back]:
-  "strict_sorted (in_traverse_keys t) \<longleftrightarrow> tree_sorted t"
-@proof @induct t @qed
-
-lemma in_traverse_fst [rewrite]:
-  "map fst (in_traverse t) = in_traverse_keys t"
+lemma inorder_sorted [rewrite_back]:
+  "strict_sorted (in_traverse t) \<longleftrightarrow> tree_sorted t"
 @proof @induct t @qed
 
 (* Use definition in terms of in_traverse from now on. *)
-setup {* fold del_prfstep_thm (@{thms tree_set_keys.simps} @ @{thms tree_sorted.simps}) *}
+setup {* fold del_prfstep_thm (@{thms tree_set.simps} @ @{thms tree_sorted.simps}) *}
 
 section {* Invariant on the maximum *}
 
-fun tree_set :: "interval_tree \<Rightarrow> (nat \<times> nat) set" where
-  "tree_set Tip = {}"
-| "tree_set (Node l it m r) = {it} \<union> tree_set l \<union> tree_set r"
-setup {* fold add_rewrite_rule @{thms tree_set.simps} *}
-
-lemma tree_set_fst [backward]:
-  "p \<in> tree_set t \<Longrightarrow> fst p \<in> tree_set_keys t"
-@proof @induct t @qed
-
 fun tree_max_inv :: "interval_tree \<Rightarrow> bool" where
   "tree_max_inv Tip = True"
-| "tree_max_inv (Node l it m r) \<longleftrightarrow> (tree_max_inv l \<and> tree_max_inv r \<and> m = max3 (snd it) (tmax l) (tmax r))"
+| "tree_max_inv (Node l it m r) \<longleftrightarrow> (tree_max_inv l \<and> tree_max_inv r \<and> m = max3 (high it) (tmax l) (tmax r))"
 setup {* fold add_rewrite_rule @{thms tree_max_inv.simps} *}
 setup {* add_property_const @{term tree_max_inv} *}
 
 lemma tree_max_is_max [resolve]:
-  "tree_max_inv t \<Longrightarrow> it \<in> tree_set t \<Longrightarrow> snd it \<le> tmax t"
+  "tree_max_inv t \<Longrightarrow> it \<in> tree_set t \<Longrightarrow> high it \<le> tmax t"
 @proof @induct t @qed
 
 lemma tmax_exists [backward]:
-  "tree_max_inv t \<Longrightarrow> t \<noteq> Tip \<Longrightarrow> \<exists>p\<in>tree_set t. snd p = tmax t"
+  "tree_max_inv t \<Longrightarrow> t \<noteq> Tip \<Longrightarrow> \<exists>p\<in>tree_set t. high p = tmax t"
 @proof @induct t @with
   @subgoal "t = Node l it m r"
     @case "l = Tip" @with @case "r = Tip" @end
@@ -98,12 +105,9 @@ fun rotateL :: "interval_tree \<Rightarrow> interval_tree" where
   "rotateL Tip = Tip"
 | "rotateL (Node l it m Tip) = Node l it m Tip"
 | "rotateL (Node l it m (Node lr itr mr rr)) =
-  (let ml = max3 (snd it) (tmax l) (tmax lr) in
-   Node (Node l it ml lr) itr (max3 (snd itr) ml (tmax rr)) rr)"
+  (let ml = max3 (high it) (tmax l) (tmax lr) in
+   Node (Node l it ml lr) itr (max3 (high itr) ml (tmax rr)) rr)"
 setup {* fold add_rewrite_rule @{thms rotateL.simps} *}
-
-lemma rotateL_in_trav_keys [rewrite]: "in_traverse_keys (rotateL t) = in_traverse_keys t"
-@proof @case "t = Tip" @then @case "rsub t = Tip" @qed
 
 lemma rotateL_in_trav [rewrite]: "in_traverse (rotateL t) = in_traverse t"
 @proof @case "t = Tip" @then @case "rsub t = Tip" @qed
@@ -117,12 +121,9 @@ fun rotateR :: "interval_tree \<Rightarrow> interval_tree" where
   "rotateR Tip = Tip"
 | "rotateR (Node Tip it m r) = Node Tip it m r"
 | "rotateR (Node (Node ll itl ml rl) it m r) =
-   (let mr = max3 (snd it) (tmax rl) (tmax r) in
-    Node ll itl (max3 (snd itl) (tmax ll) mr) (Node rl it mr r))"
+   (let mr = max3 (high it) (tmax rl) (tmax r) in
+    Node ll itl (max3 (high itl) (tmax ll) mr) (Node rl it mr r))"
 setup {* fold add_rewrite_rule @{thms rotateR.simps} *}
-
-lemma rotateR_in_trav_keys [rewrite]: "in_traverse_keys (rotateR t) = in_traverse_keys t"
-@proof @case "t = Tip" @then @case "lsub t = Tip" @qed
 
 lemma rotateR_in_trav [rewrite]: "in_traverse (rotateR t) = in_traverse t"
 @proof @case "t = Tip" @then @case "lsub t = Tip" @qed
@@ -134,54 +135,54 @@ lemma rotateR_max_inv [forward]: "tree_max_inv t \<Longrightarrow> tree_max_inv 
 
 section {* Insertion on trees *}
 
-fun tree_insert :: "nat \<times> nat \<Rightarrow> interval_tree \<Rightarrow> interval_tree" where
-  "tree_insert (a, b) Tip = Node Tip (a, b) b Tip"
-| "tree_insert (a, b) (Node l (c, d) m r) =
-    (if a = c then Node l (c, d) m r
-     else if a < c then
-       let l' = tree_insert (a, b) l in
-           Node l' (c, d) (max3 d (tmax l') (tmax r)) r
+fun tree_insert :: "nat interval \<Rightarrow> interval_tree \<Rightarrow> interval_tree" where
+  "tree_insert x Tip = Node Tip x (high x) Tip"
+| "tree_insert x (Node l y m r) =
+    (if x = y then Node l y m r
+     else if x < y then
+       let l' = tree_insert x l in
+           Node l' y (max3 (high y) (tmax l') (tmax r)) r
      else
-       let r' = tree_insert (a, b) r in
-           Node l (c, d) (max3 d (tmax l) (tmax r')) r')"
+       let r' = tree_insert x r in
+           Node l y (max3 (high y) (tmax l) (tmax r')) r')"
 setup {* fold add_rewrite_rule @{thms tree_insert.simps} *}
 
-lemma tree_insert_in_traverse_keys [rewrite]:
-  "tree_sorted t \<Longrightarrow> in_traverse_keys (tree_insert (a, b) t) = ordered_insert a (in_traverse_keys t)"
+lemma tree_insert_in_traverse [rewrite]:
+  "tree_sorted t \<Longrightarrow> in_traverse (tree_insert x t) = ordered_insert x (in_traverse t)"
 @proof @induct t @qed
 
 lemma tree_insert_on_set [rewrite]:
-  "tree_sorted t \<Longrightarrow> tree_set_keys (tree_insert (a, b) t) = {a} \<union> tree_set_keys t" by auto2
+  "tree_sorted t \<Longrightarrow> tree_set (tree_insert it t) = {it} \<union> tree_set t" by auto2
 
 lemma tree_insert_sorted [backward]:
-  "tree_sorted t \<Longrightarrow> tree_sorted (tree_insert (a, b) t)" by auto2
+  "tree_sorted t \<Longrightarrow> tree_sorted (tree_insert x t)" by auto2
 
 lemma tree_insert_max_inv:
-  "tree_max_inv t \<Longrightarrow> tree_max_inv (tree_insert (a, b) t)"
+  "tree_max_inv t \<Longrightarrow> tree_max_inv (tree_insert x t)"
 @proof @induct t @qed
 
 section {* Search on interval trees *}
 
-fun is_overlap :: "nat \<times> nat \<Rightarrow> nat \<times> nat \<Rightarrow> bool" where
-  "is_overlap (a, b) (c, d) \<longleftrightarrow> (b \<ge> c \<or> d \<ge> a)"
+fun is_overlap :: "nat interval \<Rightarrow> nat interval \<Rightarrow> bool" where
+  "is_overlap (Interval a b) (Interval c d) \<longleftrightarrow> (b \<ge> c \<or> d \<ge> a)"
 setup {* add_rewrite_rule @{thm is_overlap.simps} *}
 
-fun tree_search :: "interval_tree \<Rightarrow> nat \<times> nat \<Rightarrow> bool" where
-  "tree_search Tip (a, b) = False"
-| "tree_search (Node l (c, d) m r) (a, b) =
-   (if is_overlap (a, b) (c, d) then True
-    else if l \<noteq> Tip \<and> tmax l \<ge> a then tree_search l (a, b)
-    else tree_search r (a, b))"
+fun tree_search :: "interval_tree \<Rightarrow> nat interval \<Rightarrow> bool" where
+  "tree_search Tip x = False"
+| "tree_search (Node l y m r) x =
+   (if is_overlap x y then True
+    else if l \<noteq> Tip \<and> tmax l \<ge> low x then tree_search l x
+    else tree_search r x)"
 setup {* fold add_rewrite_rule @{thms tree_search.simps} *}
 
 fun tree_interval_inv :: "interval_tree \<Rightarrow> bool" where
   "tree_interval_inv Tip = True"
-| "tree_interval_inv (Node l (a, b) m r) = (a \<le> b \<and> tree_interval_inv l \<and> tree_interval_inv r)"
+| "tree_interval_inv (Node l (Interval a b) m r) = (a \<le> b \<and> tree_interval_inv l \<and> tree_interval_inv r)"
 setup {* fold add_rewrite_rule @{thms tree_interval_inv.simps} *}
 
 lemma tree_search_correct [rewrite]:
   "tree_sorted t \<Longrightarrow> tree_interval_inv t \<Longrightarrow> tree_max_inv t \<Longrightarrow> a \<le> b \<Longrightarrow>
-   tree_search t (a, b) \<longleftrightarrow> (\<exists>p\<in>tree_set t. is_overlap (a, b) p)"
+   tree_search t (Interval a b) \<longleftrightarrow> (\<exists>p\<in>tree_set t. is_overlap (Interval a b) p)"
 @proof @induct t @qed
 
 end
